WIP

src/tlogic/IndexedInvariants.v
@@ -18,12 +18,16 @@ Section INVARIANT_SET.
     ; inhabitant_eq : prop inhabitant = P
     }.
 
-  Definition InvSetRA (Var : Type) : URA.t := (Auth.t (positive ==> URA.agree Var))%ra.
+  Definition InvSetRA (Vars : index -> Type) (n : index) : URA.t :=
+    (Auth.t (positive ==> URA.agree (Vars n)))%ra.
 
   (* Definition IInvSetRA (Vars : index -> Type) : URA.t := (@URA.pointwise_dep index (fun n => InvSetRA (Vars n)))%ra. *)
   (* Polymorphic Definition IInvSetRA (Vars : index -> Type) : URA.t := (@URA.pointwise_dep index (fun n => InvSetRA (Vars n)))%ra. *)
   (* Polymorphic Definition IInvSetRA (Var : Type) : URA.t := (index ==> InvSetRA Var)%ra. *)
-  Definition IInvSetRA (Var : Type) : URA.t := (index ==> InvSetRA Var)%ra.
+  (* Definition IInvSetRA (Var : Type) : URA.t := (index ==> InvSetRA Var)%ra. *)
+
+  Definition IInvSetRA (Vars : index -> Type) : URA.t :=
+    @URA.pointwise_dep index (InvSetRA Vars).
 
   Global Instance InvSet_top (Var : Type) : InvSet Var :=
     {| prop := fun (_ : Var) => (⌜True⌝)%I |}.
@@ -32,6 +36,133 @@ Section INVARIANT_SET.
     {| prop := fun (_ : Var) => (⌜False⌝)%I |}.
 
 End INVARIANT_SET.
+
+Section PWDEP.
+
+  Lemma pointwise_dep_updatable
+        A (Ms : A -> URA.t)
+        (f0 f1 : @URA.pointwise_dep A Ms)
+        (UPD : forall a, URA.updatable (f0 a) (f1 a))
+    :
+    URA.updatable f0 f1.
+  Proof.
+    ii. ur. i. ur in H. specialize (H k).
+    eapply (UPD k); eauto.
+  Qed.
+
+  Lemma pointwise_dep_updatable_set
+        A (Ms : A -> URA.t)
+        (f : @URA.pointwise_dep A Ms)
+        (P : forall (a : A), (Ms a) -> Prop)
+        (UPD: forall a, URA.updatable_set (f a) (P a))
+    :
+    URA.updatable_set f (fun f' => forall a, P a (f' a)).
+  Proof.
+    ii. hexploit (Axioms.choice (fun a m => P a m /\ URA.wf (m ⋅ ctx a))).
+    { i. eapply (UPD x). ur in WF. auto. }
+    i. des. exists f0. splits; auto.
+    { i. specialize (H a). des. auto. }
+    { ur. i. specialize (H k). des. auto. }
+  Qed.
+
+  Program Definition maps_to_res_dep {A : Type} {Ms : A -> URA.t} (a : A) (m : Ms a)
+    : @URA.pointwise_dep A Ms.
+  Proof.
+    ii. destruct (Axioms.excluded_middle_informative (k = a)).
+    - subst k. exact m.
+    - exact ε.
+  Defined.
+
+  Lemma maps_to_res_dep_eq
+        A (Ms : A -> URA.t)
+        (a : A)
+        (m : Ms a)
+    :
+    (@maps_to_res_dep A Ms a m) a = m.
+  Proof.
+    unfold maps_to_res_dep. des_ifs. unfold eq_rect_r.
+    rewrite <- Eqdep.EqdepTheory.eq_rect_eq. auto.
+  Qed.
+
+  Lemma maps_to_res_dep_neq
+        A (Ms : A -> URA.t)
+        (a b : A)
+        (m : Ms a)
+    :
+    a <> b -> (@maps_to_res_dep A Ms a m) b = ε.
+  Proof.
+    i. unfold maps_to_res_dep. des_ifs.
+  Qed.
+
+  Lemma maps_to_res_dep_add
+        A (Ms : A -> URA.t)
+        (a : A)
+        (m0 m1 : Ms a)
+    :
+    @maps_to_res_dep _ Ms a m0 ⋅ @maps_to_res_dep _ Ms a m1 = @maps_to_res_dep _ Ms a (m0 ⋅ m1).
+  Proof.
+    extensionalities a'. unfold URA.add at 1. unseal "ra". ss.
+    destruct (Axioms.excluded_middle_informative (a' = a)).
+    - subst a'. rewrite ! @maps_to_res_dep_eq. auto.
+    - rewrite ! @maps_to_res_dep_neq; auto. apply URA.unit_id.
+  Qed.
+
+  Lemma maps_to_res_dep_updatable
+        A (Ms : A -> URA.t)
+        (a : A)
+        (m0 m1 : Ms a)
+        (UPD: URA.updatable m0 m1)
+    :
+    URA.updatable (@maps_to_res_dep A Ms a m0) (@maps_to_res_dep A Ms a m1).
+  Proof.
+    
+        
+
+  Lemma maps_to_updatable A (M: URA.t)
+        (a: A) (m0 m1: M)
+        (UPD: URA.updatable m0 m1)
+    :
+    URA.updatable (maps_to_res a m0) (maps_to_res a m1).
+  Proof.
+    eapply pointwise_updatable. i.
+    unfold maps_to_res. des_ifs.
+  Qed.
+
+  Lemma maps_to_updatable_set A (M: URA.t)
+        (a: A) (m: M) (P: M -> Prop)
+        (UPD: URA.updatable_set m P)
+    :
+    URA.updatable_set
+      (maps_to_res a m)
+      (fun f => exists (m1: M), f = maps_to_res a m1 /\ P m1).
+  Proof.
+    eapply updatable_set_impl; cycle 1.
+    { eapply pointwise_updatable_set.
+      instantiate (1:= fun a' m' => (a' = a -> P m') /\ (a' <> a -> m' = URA.unit)).
+      ii. unfold maps_to_res in WF. des_ifs.
+      { exploit UPD; eauto. i. des. esplits; eauto. ss. }
+      { exists URA.unit. splits; ss. }
+    }
+    { i. ss. exists (r a). splits; auto.
+      { extensionality a'. unfold maps_to_res. des_ifs.
+        specialize (H0 a'). des. auto.
+      }
+      { specialize (H0 a). des. auto. }
+    }
+  Qed.
+
+  Definition map_update {A} {M: URA.t}
+             (f: (A ==> M)%ra) a m :=
+    fun a' => if excluded_middle_informative (a' = a)
+              then m
+              else f a'.
+
+(* maps_to_res =  *)
+(* λ (A : Type) (M : URA.t) (a : A) (m : M) (a' : A), *)
+(*   if Axioms.excluded_middle_informative (a' = a) then m else ε *)
+(*      : ∀ (A : Type) (M : URA.t), A → M → (A ==> M)%ra *)
+
+End PWDEP.
 
 Section PCM_OWN.
 
@@ -43,7 +174,7 @@ Section PCM_OWN.
   Definition OwnD `{@GRA.inG (index ==> Gset.t)%ra Σ} (n : index) (D : gset positive) :=
     OwnM (@maps_to_res index Gset.t n (Some D)).
 
-  Definition OwnI_white {Var} (n : index) (i : positive) (p : Var) : IInvSetRA Var :=
+  Definition OwnI_white {Vars} (n : index) (i : positive) (p : Var) : IInvSetRA Vars :=
     @maps_to_res index (Auth.t (positive ==> URA.agree Var))%ra
                  n (Auth.white (@maps_to_res positive (URA.agree Var) i (Some (Some p)))).
 
